adding comments

Cast.v
@@ -1,3 +1,9 @@
+(******************************************************)
+(*                    Cocasse                         *)
+(* A library for Gradual Certified Programming in Coq *)
+(* Authors: Nicolas Tabareau and Eric Tanter          *)
+(******************************************************)
+
 Require Export Unicode.Utf8_core.
 Add LoadPath "." as Casts.
 Require Import String Decidable Showable.
@@ -6,10 +12,14 @@ Notation "x .1" := (proj1_sig x) (at level 3).
 Notation "x .2" := (proj2_sig x) (at level 3).
 Notation " ( x ; p ) " := (exist _ x p).
 
+(* Cast for subset types {a : A | P a}, when the property P is decidable *)
+
+(* errors are represented by the failed cast axiom *)
+
 Axiom failed_cast : 
   forall {A:Type} {P : A -> Prop} (a:A) {msg1:string} (msg2: Prop), {a : A | P a}.
 
-Definition cast (A:Type) `{Showable A} (P : A -> Prop) 
+Definition cast (A:Type) `{Show A} (P : A -> Prop) 
   (dec : forall a, Decidable (P a)) : A -> {a : A | P a} :=
 fun a: A => 
   match dec a with
@@ -19,46 +29,43 @@ fun a: A =>
 
 Notation "?" := (cast _ _ _).
 
-Definition cast_fun_range (A B : Type) `{Showable B} (P : B -> Prop) 
+(* Cast for dependent functions *)
+
+Definition cast_fun_range (A B : Type) `{Show B} (P : B -> Prop) 
   (dec : forall b, Decidable (P b)) :
     (A -> B) -> A -> {b : B | P b} :=
   fun f a => ? (f a).
 Notation "?>" := (cast_fun_range _ _ _ _).
 
-Definition cast_fun_dom (A B : Type) `{Showable A} (P: A -> Prop) 
+Definition cast_fun_dom (A B : Type) `{Show A} (P: A -> Prop) 
   (dec: forall a, Decidable (P a)) :
     ({a : A | P a} -> B)  -> A -> B :=
   fun f a => f (? a).
 Notation "<?" := (cast_fun_dom _ _ _ _).
 
-
-Definition cast_forall_range (A: Type) (B: A -> Type) `{forall a, Showable (B a)}
+Definition cast_forall_range (A: Type) (B: A -> Type) `{forall a, Show (B a)}
   (P : forall a:A, B a -> Prop) 
   (dec : forall a (b : B a), Decidable (P a b)) :
     (forall a: A, B a) -> forall a: A, {b : B a | P a b} :=
   fun f a => ? (f a).
 Notation "??>" := (cast_forall_range _ _ _ _).
 
-
-Axiom failed_cast_type : 
-  forall {A:Type} `{Showable A} {P : A -> Prop} {a: A} (msg:Prop),
+Axiom failed_cast_proj1 : 
+  forall {A:Type} `{Show A} {P : A -> Prop} {a: A} (msg:Prop),
     (failed_cast (P:=P) a (msg1 := show a) msg).1 = a.
 
-Definition hide_cast (A: Type) (P: A -> Prop) (B: A -> Type) `{Showable A}
+Definition hide_cast (A: Type) (P: A -> Prop) (B: A -> Type) `{Show A}
            (dec: forall a, Decidable (P a)) (a:A): B (? a).1 -> B a.
 Proof.
   unfold cast. case (dec a); intro p.
   - exact (fun b => b).
-  - exact (fun b => eq_rect _ _ b _ (failed_cast_type (P a))).
+  - exact (fun b => eq_rect _ _ b _ (failed_cast_proj1 (P a))).
 Defined.
 
 Notation "[?]" := (hide_cast _ _ _ _ _).
 
-
-Definition cast_forall_dom (A: Type) (P: A -> Prop) `{Showable A}
+Definition cast_forall_dom (A: Type) (P: A -> Prop) `{Show A}
            (B: A -> Type) (dec: forall a, Decidable (P a)) :
    (forall x: {a : A | P a}, B x.1)  -> (forall a : A, B a) :=
   fun f a => [?] (f (? a)).
 Notation "<??" := (cast_forall_dom _ _ _ _).
-
-
