Showable.v
@@ -1,12 +1,24 @@
-Require Import String. 
+(******************************************************)
+(*                    Cocasse                         *)
+(* A library for Gradual Certified Programming in Coq *)
+(* Authors: Nicolas Tabareau and Eric Tanter          *)
+(******************************************************)
 
-Class Showable (A :Type) := { show : A -> string }.
+                                                 
+Require Import String.
+
+(* The Show Class, similar to Haskell Show Class  *)
+
+Class Show (A :Type) := { show : A -> string }.
 
 Local Open Scope string_scope.
 
-Instance show_nat : Showable nat.
-econstructor. intro n ; induction n.
-exact "0". exact ("S ("++IHn++")").
-Defined.
+Instance show_nat : Show nat :=
+  {| show := fix _show_nat n :=
+       match n with
+         | 0 => "0"
+         | S n0 => "S (" ++ _show_nat n0 ++ ")"
+       end
+  |}.
 
 Definition not_implemented := "not implemented".
