Decidable.v
@@ -1,21 +1,22 @@
-(** printing {| $\{|$*)
-(** printing |} $|\}$*)
+(******************************************************)
+(*                    Cocasse                         *)
+(* A library for Gradual Certified Programming in Coq *)
+(* Authors: Nicolas Tabareau and Eric Tanter          *)
+(******************************************************)
 
-(* begin hide *)
 Require Import Bool List Le.
 
-Set Implicit Arguments.
+(* The Decidable Class, as defined in https://github.com/HoTT/HoTT *)
+(* We are defining it here to be independent of the Coq/HoTT library *)
 
-(* end hide *)
-
-(** The [Decidable] type class: *)
+(* We can not use the Decidable class of Coq because its definition *)
+(* is in Prop (using \/) instead of Type (using +) *)
 
 Class Decidable (A : Prop) := dec : A + (~ A).
 
 Arguments dec A {_}.
 
-
-(** ** Basic boolean reflection *)
+Set Implicit Arguments.
 
 Instance Decidable_bool (t : bool) : Decidable (Is_true t) :=
   match t with
@@ -23,26 +24,20 @@ Instance Decidable_bool (t : bool) : Decidable (Is_true t) :=
     | false => inr id
   end.
 
-(** ** Boolean reflection with proven relation to a proposition 
- %\label{app:bool_refl}%
-*)
+(* Connexion to a boolean version of decidable as in *)
 
 Class Decidable_relate (P : Prop) := {
   Decidable_witness : bool;
   Decidable_spec : Decidable_witness = true <-> P
 }.
 
-
 Instance Dec_relate_Decidable P (HP: Decidable_relate P) : 
   Decidable P.
-(* begin show *)
 destruct HP as [witness spec]. destruct witness.
 - left. exact (proj1 spec eq_refl).
 - right. intro p. pose (proj2 spec p). inversion e.
 Defined.
-(* end show *)
 
-(*begin hide *)
 Definition Decidable_Dec_relate P (HP: Decidable P) :
   Decidable_relate P.
 case HP; intro p.
@@ -50,35 +45,21 @@ case HP; intro p.
 - refine {| Decidable_witness := false |}. split; auto.
   intro e; inversion e.
 Defined.
-(* end hide *)
 
-(* begin hide *)
-(* That instance is good to show the equivalence between the styles of decidability, 
-but introduces infinite loops in type class resolution *)
-Reset Decidable_Dec_relate.
-(* end hide *)
-
-(** ** Decidable equality *)
-
-(** A type class for types with decidable equality: *)
+(* Dedicated class for dealing with decidable equality *)
 
 Class EqDecidable (A : Type) := { 
   eq_dec : forall a b : A, Decidable (a = b) 
 }.
 
-(** *** Instances for [bool] *)
-
-(* begin show *)
 Instance Decidable_eq_bool : forall (x y : bool), Decidable (eq x y).
 intros. destruct x, y; try (left ;reflexivity); 
         try (right; intro H; inversion H).
 Defined.
-(* end show *)
 
 Instance EqDecidable_bool : EqDecidable bool := 
   { eq_dec := Decidable_eq_bool }.
 
-(** *** Instances for [nat] *)
 
 Instance Decidable_eq_nat : forall (x y : nat), Decidable (eq x y).
 induction x.
@@ -94,13 +75,10 @@ Defined.
 Instance EqDecidable_nat : EqDecidable nat := 
   { eq_dec := Decidable_eq_nat }.
 
-
-
-(** *** Instances for [list] *)
+(* Instances for list *)
 
 Instance Decidable_eq_list : forall A (HA: EqDecidable A) 
   (x y: list A), Decidable (eq x y).
-(* begin show *)
 intros A HA. induction x.
 - destruct y.
   + left; reflexivity.
@@ -115,17 +93,28 @@ intros A HA. induction x.
     * right. unfold not in *. 
       intro Hc. inversion Hc. exact (H H1).
 Defined.
-(* end show *)
 
 Instance EqDecidable_list : 
   forall A (HA: EqDecidable A), EqDecidable (list A) := 
     { eq_dec := Decidable_eq_list HA }.
 
-(** *** Instances for [option] *)
+
+Instance Decidable_le_nat : forall (x y : nat), Decidable (x <= y).
+induction x.
+- destruct y.
+ + left ;reflexivity.
+ + left. apply le_S, le_0_n. 
+- induction y.
+  + right. apply le_Sn_0.
+  + case (IHx y). intro H. left. exact (le_n_S _ _ H).
+    intro H; right. intro. apply H. exact (le_S_n _ _ H0). 
+Defined.
+
+
+(* Instances for option *)
 
 Instance Decidable_eq_option : forall A (HA: EqDecidable A) 
   (x y: option A), Decidable (eq x y).
-(* begin show *)
 intros. destruct x; destruct y.
 - case (eq_dec a a0); intro H.
   + left. rewrite H. reflexivity.
@@ -135,24 +124,21 @@ intros. destruct x; destruct y.
 - right. unfold not. intro Hc. inversion Hc.
 - left. reflexivity.
 Defined.
-(* end show *)
 
 Instance EqDecidable_option :
   forall A (HA: EqDecidable A), EqDecidable (option A) := 
     { eq_dec := Decidable_eq_option HA }.
 
-(** ** Logical combination instances *)
+(* Logical combination instances *)
 
 Instance Decidable_and P Q (HP : Decidable P) 
  (HQ : Decidable Q) : Decidable (P /\ Q).
-(* begin show *)
 destruct HP.
 - destruct HQ. 
   + exact (inl (conj p q)).
   + apply inr. intro H. exact (n (proj2 H)).
 - apply inr. intro H. exact (n (proj1 H)).
 Defined.
-(* end show *)
 
 Instance Decidable_or P Q (HP : Decidable P)
         (HQ : Decidable Q) : Decidable (P \/ Q).
@@ -183,39 +169,7 @@ Instance Decidable_True : Decidable True := inl I.
 
 Instance Decidable_False : Decidable False := inr id.
 
-(** ** Some arithmetic *)
-
-Instance Decidable_le_nat : forall (x y : nat), Decidable (x <= y).
-(* begin show *)
-induction x.
-- destruct y.
- + left ;reflexivity.
- + left. apply le_S, le_0_n. 
-- induction y.
-  + right. apply le_Sn_0.
-  + case (IHx y). intro H. left. exact (le_n_S _ _ H).
-    intro H; right. intro. apply H. exact (le_S_n _ _ H0). 
-Defined.
-(* end show *)
-
-(** ** Decidability of proven properties *)
+(* Decidability of proven properties *)
 
 Instance Decidable_proven (P : Prop) (ev :  P):  Decidable P :=
   inl ev.
-
-
-(* Instance Decidable_and_right (P Q : Prop) *)
-(*   (ev: P) (HQ : Decidable Q) : *)
-(*     Decidable (P /\ Q). *)
-(* case HQ; intro H. *)
-(* - left. exact (conj ev H). *)
-(* - right. intro. destruct H0. exact (H H1). *)
-(* Defined. *)
-
-(* Instance Decidable_and_left (P Q : Prop) *)
-(*   (HP : Decidable P) (ev: Q)  : *)
-(*     Decidable (P /\ Q). *)
-(* case HP; intro H. *)
-(* - left. exact (conj H ev). *)
-(* - right. intro. destruct H0. exact (H H0). *)
-(* Defined. *)
