Examples_hs.v
@@ -1,9 +1,20 @@
+(******************************************************)
+(*                    Cocasse                         *)
+(* A library for Gradual Certified Programming in Coq *)
+(* Authors: Nicolas Tabareau and Eric Tanter          *)
+(******************************************************)
+
 Require Export Unicode.Utf8_core.
 Add LoadPath "." as Casts.
 
 Require Import Cast Decidable Showable List Ascii String.
 
 Local Open Scope string_scope.
+
+(* simple examples, with extraction to Haskell code *)
+(* The extraction does not make use of Show because of *)
+(* some issues with extraction of String to Haskell *)
+
 
 Definition x_not_ok := 1.
            
@@ -32,31 +43,3 @@ Extract Constant failed_cast =>
      "\ a s -> Prelude.error (""Cast has failed"" Prelude.++ (Prelude.show s))".
 Extraction "test.hs" client.
 
-(** ** A more involved example: casting lists *)
-
-Definition cast_list (A: Type) `{Showable A} (P : A -> Prop) 
-  (dec : forall a, Decidable (P a)): 
-    list A -> list {a : A | P a} := map ?.
-
-Notation "?::" := (cast_list _ _ _).
-
-Definition list_of_3: list {n:nat | n = 3} := ?:: (3 :: 2 :: 1 :: nil).
-
-Eval compute in list_of_3.
-
-
-Definition top_succ : nat -> {n:nat | n < 10} := ?> S.
-
-
-Eval compute in top_succ 6.
-
-Eval compute in top_succ 9.
-
-
-
-Definition foo (x: {n:nat | n > 0 }) := x.1.
-
-Extraction foo.
-
-Definition gee := <? foo.
-Extraction gee.
