compiler.v
@@ -1,3 +1,9 @@
+(******************************************************)
+(*                    Cocasse                         *)
+(* A library for Gradual Certified Programming in Coq *)
+(* Authors: Nicolas Tabareau and Eric Tanter          *)
+(******************************************************)
+
 Require Export Unicode.Utf8_core.
 Add LoadPath "." as Casts.
 Require Import Cast Decidable Showable String.
@@ -9,6 +15,8 @@ Notation "??>" := (cast_forall_range _ _ _ _).
 Notation "x .1" := (proj1_sig x) (at level 3).
 Notation "x .2" := (proj2_sig x) (at level 3).
 Notation " ( x ; p ) " := (exist _ x p).
+
+(* Main example of the paper, a correct compuiler *)
 
 Inductive binop : Set := Plus | Minus | Times.
 
@@ -40,7 +48,7 @@ Fixpoint evalExp (e: exp) : nat :=
 Eval simpl in evalExp (Const 42).
 Eval simpl in evalExp (Binop Times (Binop Plus (Const 2) (Const 2)) (Const 7)).
 
-Instance show_exp : Showable exp := {| show := fun _ => not_implemented|}.
+Instance show_exp : Show exp := {| show := fun _ => not_implemented|}.
 
 Definition e1 : {e: exp | evalExp e < 10} := ? (Binop Plus (Const 2) (Const 3)).
 (* end hide *)
@@ -71,7 +79,7 @@ Definition runInstr (i: instr) (s: stack): option stack :=
       end
   end.
 
-(** %\noindent% Running a program simply executes each instruction, recursively: *)
+(** Running a program simply executes each instruction, recursively: *)
 
 Fixpoint runProg (p: prog) (s: stack): option stack :=
   match p with
@@ -82,14 +90,7 @@ Fixpoint runProg (p: prog) (s: stack): option stack :=
                  end
   end.
 
-(* begin hide *)
 Eval compute in runProg ((iConst 2) :: (iConst 4) :: (iBinop Times) :: nil) nil.
-(* end hide *)
-
-
-(**  ** The compiler 
-
-We can now turn to the compiler, which is a recursive function that produces a program given an expression: *)
 
 Fixpoint compile (e: exp) : prog :=
   match e with
@@ -97,69 +98,23 @@ Fixpoint compile (e: exp) : prog :=
   | Binop b e1 e2 => compile e1 ++ compile e2 ++ iBinop b :: nil
   end. (* bug - compilation is correct only for commutative binops *)
 
-(** %\noindent \emph{Hint: there is a bug!} *) 
-
-(** ** Correct?
-%\label{sct:correct}%
-
-Of course, one would like to be sure that [compile] is a %{\em correct}% compiler. The traditional way of certifying the compiler is to state and prove a correctness theorem. In CPDT, the compiler correctness is stated as follows: *)
-
-Theorem compile_correct : forall (e: exp),
-  runProg (compile e) nil = Some (evalExp e :: nil).
-
-(* begin hide *)
-Abort.
-(* end hide *)
-
-
-(** %\vspace{2mm}% It turns out that the theorem cannot be proven directly by induction on expressions because of the use of [nil] in the statement of the theorem: the induction hypotheses are not useful. Instead, one has to state a generalized version of the theorem, whose proof does go by induction, and then prove [compile_correct] as a corollary%~\cite{cpdt}%. *)
-
-(**
-Instead of going into such a burden as soon as the compiler is defined, one may want to assert correctness and have it checked dynamically. With our framework, it is possible to simply cast the compiler to a correct compiler.
-
-Given a definition of [compiler], [compile_correct] is undecidable because it quantifies over all expressions. This being said, it is possible to check that the compiler is "apparently" correct by checking that it produces correct programs whenever it is used. We therefore define what a "correct program" (for a given source expression) is: %\\[2mm]%  *)
-
-(* WHY DO I NEED THE ABOVE HACKERY TO GET A PROPER LAYOUT? MISTERY... *)
 
 Definition correct_prog (e: exp) (p: prog) : Prop := 
   runProg p nil = Some (evalExp e :: nil).
 
-(** To support casting to [correct_prog], Coq must be able to build evidence that the property is decidable. But as mentioned in Section%~\ref{sec:decidable}% and further explained in Section%~\ref{sec:leveraging}%, the evidence is automatically computed by the type class resolution, which allows us to define the (supposedly) correct compiler simply as:
- *)
-(* There are different ways to achieve this, which we explore in this and the following sections. A first solution is to define a decision procedure: *) 
-(*begin hide *)
 Definition b_correct_prog (e: exp) (p: prog) : bool :=
   match runProg p nil with
     | Some (v :: nil) => Nat.eqb v (evalExp e)
     | _ => false
   end.
-(*end hide *)
 
-Instance show_prog : Showable prog := {| show := fun _ => not_implemented|}.
+Instance show_prog : Show prog := {| show := fun _ => not_implemented|}.
 
 Definition correct_compiler :
   forall e:exp, { p: prog | correct_prog e p } := ??> compile.
 
-
-(* We still need to lift this decision procedure to the property level. The simplest way to do so is to assert compiler correctness based on reflecting [b_correct_prog] directly as a property: *)
-(* Definition correct_prog_r (e: exp) (p: prog) : Prop :=  *)
-(*   Is_true (b_correct_prog e p). *)
-(* %\noindent% We can now define a correct compiler by casting [compile]: *)
-(* Definition correct_compiler : *)
-  (* forall e:exp, { p: prog | correct_prog_r e p } := ??> compile. *)
-
-(**  We can now exercise [correct_prog]. The following evaluation succeeds: *)
-
 Eval compute in 
   correct_compiler (Binop Plus (Const 2) (Const 2)).
-
-(** 
-<<
-= (iConst 2 :: iConst 2 :: iBinop Plus :: nil; 
-   eq_refl)
-: {p : prog | correct_prog ...}
->>
-*)
 
 (** However, the cast fails when using a (non-commutative!) subtraction operation: *)
 
